<?xml version="1.0"?>
<rdf:RDF xmlns="http://w3id.org/reshare/ontology/0.3/"
     xml:base="http://w3id.org/reshare/ontology/0.3/"
     xmlns:dc="http://purl.org/dc/elements/1.1/"
     xmlns:ns="http://www.w3.org/2003/06/sw-vocab-status/ns#"
     xmlns:owl="http://www.w3.org/2002/07/owl#"
     xmlns:rdf="http://www.w3.org/1999/02/22-rdf-syntax-ns#"
     xmlns:xml="http://www.w3.org/XML/1998/namespace"
     xmlns:xsd="http://www.w3.org/2001/XMLSchema#"
     xmlns:rdfs="http://www.w3.org/2000/01/rdf-schema#">
    <owl:Ontology rdf:about="http://w3id.org/reshare/ontology/0.3/">
        <dc:description>The ReShare (Reliable Data Sharing Through Digital Transmission contracts) vocabulary, described using W3C RDF Schema and the Web Ontology Language.</dc:description>
        <dc:language>en</dc:language>
        <dc:title>ReShare Vocabulary v0.3</dc:title>
        <owl:priorVersion>http://w3id.org/reshare/ontology/0.2/</owl:priorVersion>
        <owl:versionInfo>0.3</owl:versionInfo>
    </owl:Ontology>
    


    <!-- 
    ///////////////////////////////////////////////////////////////////////////////////////
    //
    // Annotation properties
    //
    ///////////////////////////////////////////////////////////////////////////////////////
     -->


    


    <!-- http://purl.org/dc/elements/1.1/description -->


    <owl:AnnotationProperty rdf:about="http://purl.org/dc/elements/1.1/description"/>
    


    <!-- http://purl.org/dc/elements/1.1/language -->


    <owl:AnnotationProperty rdf:about="http://purl.org/dc/elements/1.1/language"/>
    


    <!-- http://purl.org/dc/elements/1.1/title -->


    <owl:AnnotationProperty rdf:about="http://purl.org/dc/elements/1.1/title"/>
    


    <!-- http://www.w3.org/2003/06/sw-vocab-status/ns#term_status -->


    <owl:AnnotationProperty rdf:about="http://www.w3.org/2003/06/sw-vocab-status/ns#term_status"/>
    


    <!-- 
    ///////////////////////////////////////////////////////////////////////////////////////
    //
    // Object Properties
    //
    ///////////////////////////////////////////////////////////////////////////////////////
     -->


    


    <!-- http://w3id.org/reshare/ontology/0.3/#fact -->


    <owl:ObjectProperty rdf:about="http://w3id.org/reshare/ontology/0.3/#fact">
        <rdfs:domain rdf:resource="http://w3id.org/reshare/ontology/0.3/#DTC"/>
        <rdfs:range rdf:resource="http://w3id.org/reshare/ontology/0.3/#Fact"/>
        <rdfs:comment>A fact included in a DTC.</rdfs:comment>
        <rdfs:isDefinedBy rdf:resource="http://w3id.org/reshare/ontology/0.3/"/>
        <rdfs:label>has fact</rdfs:label>
        <ns:term_status>stable</ns:term_status>
    </owl:ObjectProperty>
    


    <!-- http://w3id.org/reshare/ontology/0.3/#factOrigin -->


    <owl:ObjectProperty rdf:about="http://w3id.org/reshare/ontology/0.3/#factOrigin">
        <rdfs:domain rdf:resource="http://w3id.org/reshare/ontology/0.3/#Fact"/>
        <rdfs:comment>The resource which is referenced by the fact.</rdfs:comment>
        <rdfs:isDefinedBy rdf:resource="http://w3id.org/reshare/ontology/0.3/"/>
        <rdfs:label>fact origin</rdfs:label>
        <ns:term_status>stable</ns:term_status>
    </owl:ObjectProperty>
    


    <!-- http://w3id.org/reshare/ontology/0.3/#identifies -->


    <owl:ObjectProperty rdf:about="http://w3id.org/reshare/ontology/0.3/#identifies">
        <rdfs:domain rdf:resource="http://w3id.org/reshare/ontology/0.3/#Identity"/>
        <rdfs:comment>Links an identity of a receiver or sender as part of a contract to that entity. It is best practice to use an instance of foaf:Agent as the object to this property.</rdfs:comment>
        <rdfs:isDefinedBy rdf:resource="http://w3id.org/reshare/ontology/0.3/"/>
        <rdfs:label>identifies</rdfs:label>
        <ns:term_status>stable</ns:term_status>
    </owl:ObjectProperty>
    


    <!-- http://w3id.org/reshare/ontology/0.3/#receiver -->


    <owl:ObjectProperty rdf:about="http://w3id.org/reshare/ontology/0.3/#receiver">
        <rdfs:domain rdf:resource="http://w3id.org/reshare/ontology/0.3/#DTC"/>
        <rdfs:range rdf:resource="http://w3id.org/reshare/ontology/0.3/#Receiver"/>
        <rdfs:comment>The data receiver of the underlying transmission of a DTC.</rdfs:comment>
        <rdfs:isDefinedBy rdf:resource="http://w3id.org/reshare/ontology/0.3/"/>
        <rdfs:label>receiver</rdfs:label>
        <ns:term_status>stable</ns:term_status>
    </owl:ObjectProperty>
    


    <!-- http://w3id.org/reshare/ontology/0.3/#receiverSig -->


    <owl:ObjectProperty rdf:about="http://w3id.org/reshare/ontology/0.3/#receiverSig">
        <rdfs:domain rdf:resource="http://w3id.org/reshare/ontology/0.3/#DTC"/>
        <rdfs:range rdf:resource="http://w3id.org/reshare/ontology/0.3/#Signature"/>
        <rdfs:comment>The contract signature created by the receiver of the DTC.</rdfs:comment>
        <rdfs:isDefinedBy rdf:resource="http://w3id.org/reshare/ontology/0.3/"/>
        <rdfs:label>receiver signature</rdfs:label>
        <ns:term_status>stable</ns:term_status>
    </owl:ObjectProperty>
    


    <!-- http://w3id.org/reshare/ontology/0.3/#requestedFactOrigin -->


    <owl:ObjectProperty rdf:about="http://w3id.org/reshare/ontology/0.3/#requestedFactOrigin">
        <rdfs:domain rdf:resource="http://w3id.org/reshare/ontology/0.3/#Fact"/>
        <rdfs:comment>The resource which was referenced by the receiver when initially requesting a contract. This property is used when the resource reference is updated by the sender during the contract generation handshake.</rdfs:comment>
        <rdfs:isDefinedBy rdf:resource="http://w3id.org/reshare/ontology/0.3/"/>
        <rdfs:label>requested fact origin</rdfs:label>
        <ns:term_status>stable</ns:term_status>
    </owl:ObjectProperty>
    


    <!-- http://w3id.org/reshare/ontology/0.3/#sender -->


    <owl:ObjectProperty rdf:about="http://w3id.org/reshare/ontology/0.3/#sender">
        <rdfs:domain rdf:resource="http://w3id.org/reshare/ontology/0.3/#DTC"/>
        <rdfs:range rdf:resource="http://w3id.org/reshare/ontology/0.3/#Sender"/>
        <rdfs:comment>The data source (sender) of the underlying transmission of a DTC.</rdfs:comment>
        <rdfs:isDefinedBy rdf:resource="http://w3id.org/reshare/ontology/0.3/"/>
        <rdfs:label>sender</rdfs:label>
        <ns:term_status>stable</ns:term_status>
    </owl:ObjectProperty>
    


    <!-- http://w3id.org/reshare/ontology/0.3/#senderSig -->


    <owl:ObjectProperty rdf:about="http://w3id.org/reshare/ontology/0.3/#senderSig">
        <rdfs:domain rdf:resource="http://w3id.org/reshare/ontology/0.3/#DTC"/>
        <rdfs:range rdf:resource="http://w3id.org/reshare/ontology/0.3/#Signature"/>
        <rdfs:comment>The contract signature created by the sender of the DTC.</rdfs:comment>
        <rdfs:isDefinedBy rdf:resource="http://w3id.org/reshare/ontology/0.3/"/>
        <rdfs:label>sender signature</rdfs:label>
        <ns:term_status>stable</ns:term_status>
    </owl:ObjectProperty>
    


    <!-- http://w3id.org/reshare/ontology/0.3/#sigType -->


    <owl:ObjectProperty rdf:about="http://w3id.org/reshare/ontology/0.3/#sigType">
        <rdfs:domain rdf:resource="http://w3id.org/reshare/ontology/0.3/#Signature"/>
        <rdfs:comment>The type of a contract signature. The object should be an OID URN to a cryptographic signature scheme. As of now, &apos;urn:oid:1.2.840.113549.1.1.10&apos; is considered the default value, identifying the RSASSA-PSS signature scheme as specified in PKCS #1 v2.2.</rdfs:comment>
        <rdfs:isDefinedBy rdf:resource="http://w3id.org/reshare/ontology/0.3/"/>
        <rdfs:label>signature type</rdfs:label>
        <ns:term_status>stable</ns:term_status>
    </owl:ObjectProperty>
    


    <!-- 
    ///////////////////////////////////////////////////////////////////////////////////////
    //
    // Data properties
    //
    ///////////////////////////////////////////////////////////////////////////////////////
     -->


    


    <!-- http://w3id.org/reshare/ontology/0.3/#certEncoding -->


    <owl:DatatypeProperty rdf:about="http://w3id.org/reshare/ontology/0.3/#certEncoding">
        <rdfs:domain rdf:resource="http://w3id.org/reshare/ontology/0.3/#Identity"/>
        <rdfs:range rdf:resource="http://www.w3.org/2000/01/rdf-schema#Literal"/>
        <rdfs:comment>Encoding of the (binary) certificate data object to the x509Cert property. &apos;base64&apos; is considered the default value, expressing that the (binary) certificate data which is object to the x509Cert property is encoded using Base64.</rdfs:comment>
        <rdfs:isDefinedBy rdf:resource="http://w3id.org/reshare/ontology/0.3/"/>
        <rdfs:label>certificate encoding</rdfs:label>
        <ns:term_status>stable</ns:term_status>
    </owl:DatatypeProperty>
    


    <!-- http://w3id.org/reshare/ontology/0.3/#certType -->


    <owl:DatatypeProperty rdf:about="http://w3id.org/reshare/ontology/0.3/#certType">
        <rdfs:domain rdf:resource="http://w3id.org/reshare/ontology/0.3/#Identity"/>
        <rdfs:range rdf:resource="http://www.w3.org/2000/01/rdf-schema#Literal"/>
        <rdfs:comment>The type of the certificate provided by the Identity. &apos;X509&apos;/&apos;X509-single&apos; identify single X.509 certificates in ASN.1 DER notation, and &apos;PKCS7&apos;/&apos;X509-PKCS7-chain&apos; identify an X.509 certificate chain encoded as a PKCS#7 message.</rdfs:comment>
        <rdfs:isDefinedBy rdf:resource="http://w3id.org/reshare/ontology/0.3/"/>
        <rdfs:label>certificate type</rdfs:label>
        <ns:term_status>stable</ns:term_status>
    </owl:DatatypeProperty>
    


    <!-- http://w3id.org/reshare/ontology/0.3/#customContent -->


    <owl:DatatypeProperty rdf:about="http://w3id.org/reshare/ontology/0.3/#customContent">
        <rdfs:domain rdf:resource="http://w3id.org/reshare/ontology/0.3/#DTC"/>
        <rdfs:range rdf:resource="http://www.w3.org/2000/01/rdf-schema#Literal"/>
        <rdfs:comment>The property linking a DTC to the custom content included by one of the parties. The object should be a literal with the JSON type (http://www.w3.org/1999/02/22-rdf-syntax-ns#JSON). Abstract property, use the sub-properties instead.</rdfs:comment>
        <rdfs:isDefinedBy rdf:resource="http://w3id.org/reshare/ontology/0.3/"/>
        <rdfs:label>custom content</rdfs:label>
        <ns:term_status>stable</ns:term_status>
    </owl:DatatypeProperty>
    


    <!-- http://w3id.org/reshare/ontology/0.3/#receiverCustomContent -->


    <owl:DatatypeProperty rdf:about="http://w3id.org/reshare/ontology/0.3/#receiverCustomContent">
        <rdfs:subPropertyOf rdf:resource="http://w3id.org/reshare/ontology/0.3/#customContent"/>
        <rdfs:domain rdf:resource="http://w3id.org/reshare/ontology/0.3/#DTC"/>
        <rdfs:range rdf:resource="http://www.w3.org/2000/01/rdf-schema#Literal"/>
        <rdfs:comment>The receiver&apos;s custom content.</rdfs:comment>
        <rdfs:isDefinedBy rdf:resource="http://w3id.org/reshare/ontology/0.3/"/>
        <rdfs:label>receiver custom content</rdfs:label>
        <ns:term_status>stable</ns:term_status>
    </owl:DatatypeProperty>
    


    <!-- http://w3id.org/reshare/ontology/0.3/#senderCustomContent -->


    <owl:DatatypeProperty rdf:about="http://w3id.org/reshare/ontology/0.3/#senderCustomContent">
        <rdfs:subPropertyOf rdf:resource="http://w3id.org/reshare/ontology/0.3/#customContent"/>
        <rdfs:domain rdf:resource="http://w3id.org/reshare/ontology/0.3/#DTC"/>
        <rdfs:range rdf:resource="http://www.w3.org/2000/01/rdf-schema#Literal"/>
        <rdfs:comment>The sender&apos;s custom content.</rdfs:comment>
        <rdfs:isDefinedBy rdf:resource="http://w3id.org/reshare/ontology/0.3/"/>
        <rdfs:label>sender custom content</rdfs:label>
        <ns:term_status>stable</ns:term_status>
    </owl:DatatypeProperty>
    


    <!-- http://w3id.org/reshare/ontology/0.3/#serialization -->


    <owl:DatatypeProperty rdf:about="http://w3id.org/reshare/ontology/0.3/#serialization">
        <rdfs:domain rdf:resource="http://w3id.org/reshare/ontology/0.3/#Fact"/>
        <rdfs:range rdf:resource="http://www.w3.org/2000/01/rdf-schema#Literal"/>
        <rdfs:comment>The serialization method used to create a verifiable fact checksum. Some string identifiers are defined in the specification of ReShare (see TODO: ref to ReShare)</rdfs:comment>
        <rdfs:isDefinedBy rdf:resource="http://w3id.org/reshare/ontology/0.3/"/>
        <rdfs:label>fact serialization</rdfs:label>
        <ns:term_status>stable</ns:term_status>
    </owl:DatatypeProperty>
    


    <!-- http://w3id.org/reshare/ontology/0.3/#sha256Sum -->


    <owl:DatatypeProperty rdf:about="http://w3id.org/reshare/ontology/0.3/#sha256Sum">
        <rdfs:domain rdf:resource="http://w3id.org/reshare/ontology/0.3/#Fact"/>
        <rdfs:range rdf:resource="http://www.w3.org/2000/01/rdf-schema#Literal"/>
        <rdfs:comment>A SHA-256 checksum of a fact. Should be encoded as a hex stream using the xsd:hexBinary literal type.</rdfs:comment>
        <rdfs:isDefinedBy rdf:resource="http://w3id.org/reshare/ontology/0.3/"/>
        <rdfs:label>fact checksum (sha256)</rdfs:label>
        <ns:term_status>stable</ns:term_status>
    </owl:DatatypeProperty>
    


    <!-- http://w3id.org/reshare/ontology/0.3/#sha384Sum -->


    <owl:DatatypeProperty rdf:about="http://w3id.org/reshare/ontology/0.3/#sha384Sum">
        <rdfs:domain rdf:resource="http://w3id.org/reshare/ontology/0.3/#Fact"/>
        <rdfs:range rdf:resource="http://www.w3.org/2000/01/rdf-schema#Literal"/>
        <rdfs:comment>A SHA-384 checksum of a fact. Should be encoded as a hex stream using the xsd:hexBinary literal type.</rdfs:comment>
        <rdfs:isDefinedBy rdf:resource="http://w3id.org/reshare/ontology/0.3/"/>
        <rdfs:label>fact checksum (sha384)</rdfs:label>
        <ns:term_status>stable</ns:term_status>
    </owl:DatatypeProperty>
    


    <!-- http://w3id.org/reshare/ontology/0.3/#sha512Sum -->


    <owl:DatatypeProperty rdf:about="http://w3id.org/reshare/ontology/0.3/#sha512Sum">
        <rdfs:domain rdf:resource="http://w3id.org/reshare/ontology/0.3/#Fact"/>
        <rdfs:range rdf:resource="http://www.w3.org/2000/01/rdf-schema#Literal"/>
        <rdfs:comment>A SHA-512 checksum of a fact. Should be encoded as a hex stream using the xsd:hexBinary literal type.</rdfs:comment>
        <rdfs:isDefinedBy rdf:resource="http://w3id.org/reshare/ontology/0.3/"/>
        <rdfs:label>fact checksum (sha512)</rdfs:label>
        <ns:term_status>stable</ns:term_status>
    </owl:DatatypeProperty>
    


    <!-- http://w3id.org/reshare/ontology/0.3/#sigData -->


    <owl:DatatypeProperty rdf:about="http://w3id.org/reshare/ontology/0.3/#sigData">
        <rdfs:domain rdf:resource="http://w3id.org/reshare/ontology/0.3/#Signature"/>
        <rdfs:range rdf:resource="http://www.w3.org/2000/01/rdf-schema#Literal"/>
        <rdfs:comment>The signature data, encoded as a character sequence. More information about the type and encoding can be provided with the sigType and sigEncoding properties. If Base64 is used for the character encoding, the literal type should be xsd:base64Binary.</rdfs:comment>
        <rdfs:isDefinedBy rdf:resource="http://w3id.org/reshare/ontology/0.3/"/>
        <rdfs:label>signature data</rdfs:label>
        <ns:term_status>stable</ns:term_status>
    </owl:DatatypeProperty>
    


    <!-- http://w3id.org/reshare/ontology/0.3/#sigEncoding -->


    <owl:DatatypeProperty rdf:about="http://w3id.org/reshare/ontology/0.3/#sigEncoding">
        <rdfs:domain rdf:resource="http://w3id.org/reshare/ontology/0.3/#Signature"/>
        <rdfs:range rdf:resource="http://www.w3.org/2000/01/rdf-schema#Literal"/>
        <rdfs:comment>The signature encoding. &apos;base64&apos; is considered the default value, expressing that the (binary) signature data which is object to the sigData property is encoded using Base64.</rdfs:comment>
        <rdfs:isDefinedBy rdf:resource="http://w3id.org/reshare/ontology/0.3/"/>
        <rdfs:label>signature encoding</rdfs:label>
        <ns:term_status>stable</ns:term_status>
    </owl:DatatypeProperty>
    


    <!-- http://w3id.org/reshare/ontology/0.3/#timestamp -->


    <owl:DatatypeProperty rdf:about="http://w3id.org/reshare/ontology/0.3/#timestamp">
        <rdfs:domain rdf:resource="http://w3id.org/reshare/ontology/0.3/#DTC"/>
        <rdfs:range rdf:resource="http://www.w3.org/2000/01/rdf-schema#Literal"/>
        <rdfs:comment>The timestamp of a DTC. Should be in the RFC3339 profile of ISO 8601, and should have the xsd:dateTimeStamp literal type.</rdfs:comment>
        <rdfs:isDefinedBy rdf:resource="http://w3id.org/reshare/ontology/0.3/"/>
        <rdfs:label>timestamp</rdfs:label>
        <ns:term_status>stable</ns:term_status>
    </owl:DatatypeProperty>
    


    <!-- http://w3id.org/reshare/ontology/0.3/#x509Cert -->


    <owl:DatatypeProperty rdf:about="http://w3id.org/reshare/ontology/0.3/#x509Cert">
        <rdfs:domain rdf:resource="http://w3id.org/reshare/ontology/0.3/#Identity"/>
        <rdfs:range rdf:resource="http://www.w3.org/2000/01/rdf-schema#Literal"/>
        <rdfs:comment>The public key certificate of a transmission party. Should be the full certificate chain,     excluding the root certificate, encoded as a character sequence. Further information about the certificate can be included in the certType and certEncoding properties. If Base64 is used for the character encoding, the xsd:base64Binary literal type should be used.</rdfs:comment>
        <rdfs:isDefinedBy rdf:resource="http://w3id.org/reshare/ontology/0.3/"/>
        <rdfs:label>X.509 certificate</rdfs:label>
        <ns:term_status>stable</ns:term_status>
    </owl:DatatypeProperty>
    


    <!-- 
    ///////////////////////////////////////////////////////////////////////////////////////
    //
    // Classes
    //
    ///////////////////////////////////////////////////////////////////////////////////////
     -->


    


    <!-- http://w3id.org/reshare/ontology/0.3/#DTC -->


    <owl:Class rdf:about="http://w3id.org/reshare/ontology/0.3/#DTC">
        <rdfs:comment>A Digital Transmisson Contract (DTC), used to create data immutability through bilateral signatures.</rdfs:comment>
        <rdfs:isDefinedBy rdf:resource="http://w3id.org/reshare/ontology/0.3/"/>
        <rdfs:label>Digital Transmission Contract</rdfs:label>
        <ns:term_status>stable</ns:term_status>
    </owl:Class>
    


    <!-- http://w3id.org/reshare/ontology/0.3/#Fact -->


    <owl:Class rdf:about="http://w3id.org/reshare/ontology/0.3/#Fact">
        <rdfs:comment>A resource checksum which is included in a DTC.</rdfs:comment>
        <rdfs:isDefinedBy rdf:resource="http://w3id.org/reshare/ontology/0.3/"/>
        <rdfs:label>Fact</rdfs:label>
        <ns:term_status>stable</ns:term_status>
    </owl:Class>
    


    <!-- http://w3id.org/reshare/ontology/0.3/#Identity -->


    <owl:Class rdf:about="http://w3id.org/reshare/ontology/0.3/#Identity">
        <rdfs:comment>An identity of a transmission party.</rdfs:comment>
        <rdfs:isDefinedBy rdf:resource="http://w3id.org/reshare/ontology/0.3/"/>
        <rdfs:label>Identity</rdfs:label>
        <ns:term_status>stable</ns:term_status>
    </owl:Class>
    


    <!-- http://w3id.org/reshare/ontology/0.3/#Receiver -->


    <owl:Class rdf:about="http://w3id.org/reshare/ontology/0.3/#Receiver">
        <rdfs:subClassOf rdf:resource="http://w3id.org/reshare/ontology/0.3/#Identity"/>
        <rdfs:comment>The receiver of a transmission.</rdfs:comment>
        <rdfs:isDefinedBy rdf:resource="http://w3id.org/reshare/ontology/0.3/"/>
        <rdfs:label>Receiver</rdfs:label>
        <ns:term_status>stable</ns:term_status>
    </owl:Class>
    


    <!-- http://w3id.org/reshare/ontology/0.3/#Sender -->


    <owl:Class rdf:about="http://w3id.org/reshare/ontology/0.3/#Sender">
        <rdfs:subClassOf rdf:resource="http://w3id.org/reshare/ontology/0.3/#Identity"/>
        <rdfs:comment>The data source (sender) of a transmission.</rdfs:comment>
        <rdfs:isDefinedBy rdf:resource="http://w3id.org/reshare/ontology/0.3/"/>
        <rdfs:label>Sender</rdfs:label>
        <ns:term_status>stable</ns:term_status>
    </owl:Class>
    


    <!-- http://w3id.org/reshare/ontology/0.3/#Signature -->


    <owl:Class rdf:about="http://w3id.org/reshare/ontology/0.3/#Signature">
        <rdfs:comment>A contract signature created by one of the transmission parties.</rdfs:comment>
        <rdfs:isDefinedBy rdf:resource="http://w3id.org/reshare/ontology/0.3/"/>
        <rdfs:label>Signature</rdfs:label>
        <ns:term_status>stable</ns:term_status>
    </owl:Class>
</rdf:RDF>



<!-- Generated by the OWL API (version 5.1.14) https://github.com/owlcs/owlapi/ -->


